\documentclass[12pt]{article}

\usepackage[utf8]{inputenc}
\usepackage[english, russian]{babel}
\usepackage{amsthm}

\title{Домашнее задание 1. Введение в алгебру логики}
\author{Балдин Виктор Б01-303}

\begin{document}
    \maketitle

    \begin{enumerate}
        \item Доказать, что
            \[1\oplus x_1 \oplus x_2 = (x_1 \to x_2) \wedge (x_2 \to x_1)\]
        \textbf{Доказательство: }
        \[1 \oplus x_1 \oplus x2 = \lnot(x1 \oplus x2) = x_1\leftrightarrow
        x_2\]
        \[ (x_1 \to x_2) \wedge (x_2 \to x_1) = (\lnot x_1 
        \vee x_2) \wedge (\lnot x_2 \vee x_1) = \lnot 
        x_1 \wedge \lnot x_2 \vee x_1 \wedge x_2 = x_1 \leftrightarrow x_2\]
        \qedsymbol{}
        
        \item Проверить:
        \subitem (a) \( x \wedge (y \to z) = (x \wedge y) \to
        (x \wedge z) \)
        \subitem (b) \( x \oplus (y \leftrightarrow z) = (x \oplus y) 
        \leftrightarrow (x \oplus z) \)

        \textbf{Решение:}
        \subitem (a) \( x \wedge (y \to z) = x \wedge (\lnot y \vee z)
        = x \wedge \lnot y \vee x \wedge z \neq \lnot(x \wedge y) \vee x \wedge
        z = (x \wedge y) \to (x \wedge z)\) -- \textit{ложно}
        \subitem (b) \( x \oplus (y \leftrightarrow z) = 
        \lnot(x \leftrightarrow (y \leftrightarrow z)) = 
        \lnot(x \to (y \leftrightarrow z) \wedge (y \leftrightarrow z) \to
        x) = \lnot(x \to (y \leftrightarrow z)) \vee 
        \lnot((y \leftrightarrow z) \to x) = x \wedge (y \oplus z) \vee
        (y \oplus z) \wedge x = x \wedge (y \oplus z) = \lnot ((x \wedge y)
        \leftrightarrow (x \wedge z) )\)
    \end{enumerate}
\end{document}